experiments/channels.v
@@ -1,0 +1,80 @@
+From stdpp Require Import gmap numbers countable mapset.
+
+From iris.program_logic Require Export atomic.
+From iris.proofmode Require Import proofmode tactics coq_tactics reduction.
+From iris.prelude Require Import options.
+From iris.heap_lang Require Import proofmode notation.
+
+From eIris.proofmode Require Import base reduction inductive intros.
+
+Section Channels.
+  Context `{!heapGS Σ}.
+  Notation iProp := (iProp Σ).
+  Implicit Types l nl tl lh lt : loc.
+
+
+  Local Definition tag_nil : Z := 0.
+  Local Definition tag_cons : Z := 1.
+  Local Definition tag_link : Z := 2.
+
+  (* #[debug] *)
+  EI.ind
+  Inductive is_queue : loc → loc → list val → iProp :=
+      | nill_is_queue l : l ↦ #tag_nil -∗ is_queue l l []
+      | cons_is_queue v vs l nl tl : 
+          l ↦ #tag_cons -∗ (l +ₗ 1) ↦ v -∗ (l +ₗ 2) ↦ #nl -∗ 
+          is_queue nl tl vs -∗ is_queue l tl (v :: vs)
+      | link_is_queue vs l nl tl : 
+          l ↦ #tag_cons -∗ (l +ₗ 2) ↦ #nl -∗ 
+          is_queue nl tl vs -∗ is_queue l tl vs.
+
+  Print is_queue_pre.
+
+  Definition new_queue : val := λ: <>,
+    let: "end" := AllocN #3 #() in
+    ("end" +ₗ #0) <- #tag_nil;;
+    ("end", "end").
+
+  Definition enqueue : val := λ: "t" "x",
+    let: "end" := AllocN #3 #() in
+    ("end" +ₗ #0) <- #tag_nil;;
+
+    ("t" +ₗ #1) <- "x";;
+    ("t" +ₗ #2) <- "end";;
+    ("t" +ₗ #0) <- #tag_cons;;
+
+    "end".
+
+  Definition dequeue : val :=
+    rec: "dequeue" "d" :=
+      if: !("d" +ₗ #0) = #tag_nil then
+        "dequeue" "d"
+      else if: !("d" +ₗ #0) = #tag_cons then
+        (!("d" +ₗ #2), !("d" +ₗ #1))
+      else
+        "dequeue" !("d" +ₗ #2).
+
+  Definition link_queue : val := λ: "t" "h",
+    let: "node" := !"t" in
+    let: "lh" := !"h" in
+    ("node" +ₗ #2) <- "lh";;
+    ("node" +ₗ #0) <- #tag_link;;
+    #().
+
+  Lemma new_queue_spec:
+    {{{ True }}}
+      new_queue #()
+    {{{ lh lt, RET (#lh, #lt);
+        is_queue lh lt [] }}}.
+  Proof.
+    iIntros (Φ) "_ HΦ".
+    wp_lam. wp_alloc l as "Hl /="; first by lia.
+    wp_pures.
+    iDestruct (array_cons with "Hl") as "[Hl0 Hl]".
+    iDestruct (array_cons with "Hl") as "[Hl1 Hl]".
+    iDestruct (array_cons with "Hl") as "[Hl2 Hl]".
+    rewrite !Loc.add_assoc Loc.add_0.
+    wp_store.
+    wp_pures. iModIntro. iApply "HΦ".
+    iApply nill_is_queue. by iFrame.
+  Qed.
