experiments/indtests.v
@@ -17,6 +17,15 @@ Section Tests.
   Implicit Types l : loc.
 
   EI.ind
+  Inductive is_R_MLL {A} (R : val -> A -> iProp) : val → list A → iProp :=
+      | empty_is_R_MLL : is_R_MLL R NONEV []
+      | mark_is_R_MLL v xs l tl : l ↦ (v, #true, tl) -∗ is_R_MLL R tl xs -∗ is_R_MLL R (SOMEV #l) xs
+      | cons_is_R_MLL v x xs tl l : l ↦ (v, #false, tl) -∗ R v x -∗ is_R_MLL R tl xs -∗ is_R_MLL R (SOMEV #l) (x :: xs).
+    
+  Print is_R_MLL_pre.
+  Check is_MLL_ind.
+
+  EI.ind
   Inductive is_R_list {A} (R : val → A → iProp) : 
                       val → list A → iProp :=
     | empty_is_R_list : is_R_list R NONEV []
