experiments/test.v
@@ -1,0 +1,4 @@
+Lemma test : False = True -> True.
+Proof.
+intros H. 
+Admitted.
